proof/SimProg.v
@@ -40,7 +40,7 @@ Context `{SM: SimMem.class} {SS: SimSymb.class SM}.
   Definition src (pp: t): program := List.map ModPair.src pp.
   Definition tgt (pp: t): program := List.map ModPair.tgt pp.
 
-  Definition ss_link (pp: t): option SimSymb.t := link_list (List.map ModPair.ss pp).
+  (* Definition ss_link (pp: t): option SimSymb.t := link_list (List.map ModPair.ss pp). *)
   (* ############ TODO: *)
   (* ModPair.wf mp0 /\ ModPair.wf mp1 /\ link mp0.(src) mp1.(src) = Some /\ link mp1.(tgt) mp1.(tgt) = Some *)
   (* =================> link mp0.(ss) mp1.(ss) suceeds. *)
@@ -49,7 +49,8 @@ Context `{SM: SimMem.class} {SS: SimSymb.class SM}.
 End PROGPAIR.
 End ProgPair.
 
-Hint Unfold ProgPair.sim ProgPair.src ProgPair.tgt ProgPair.ss_link.
+Hint Unfold ProgPair.sim ProgPair.src ProgPair.tgt.
+(* Hint Unfold ProgPair.ss_link. *)
 
 
 
@@ -65,59 +66,59 @@ Hint Unfold ProgPair.sim ProgPair.src ProgPair.tgt ProgPair.ss_link.
 
 
 
-Section SIM.
-Context `{SM: SimMem.class} {SS: SimSymb.class SM}.
+(* Section SIM. *)
+(* Context `{SM: SimMem.class} {SS: SimSymb.class SM}. *)
 
-  Variable pp: ProgPair.t.
-  Hypothesis SIMPROG: ProgPair.sim pp.
-  Let p_src := pp.(ProgPair.src).
-  Let p_tgt := pp.(ProgPair.tgt).
-
-
-
-  Theorem sim_link_sk
-          sk_link_src
-          (LOADSRC: p_src.(link_sk) = Some sk_link_src)
-    :
-      exists ss_link sk_link_tgt,
-        <<LOADTGT: p_tgt.(link_sk) = Some sk_link_tgt>>
-        /\ <<LINKSS: pp.(ProgPair.ss_link) = Some ss_link>> 
-        /\ <<SIMSK: SimSymb.sim_sk ss_link sk_link_src sk_link_tgt>>
-  .
-  Proof.
-    u. subst_locals.
-    ginduction pp; ii; ss.
-    eapply link_list_cons_inv in LOADSRC. des.
-    inv SIMPROG.
-    exploit IHt; eauto. intro IH; des.
-    inv H1.
-    rename sk_link_src into sk_link_link_src.
-    rename restl into sk_link_src.
-    exploit SimSymb.sim_sk_weak_enables_link; eauto.
-    { eapply SimSymb.sim_sk_sim_sk_weak; eauto. }
-    { eapply SimSymb.sim_sk_sim_sk_weak; eauto. }
-    i; des.
-    exploit SimSymb.link_preserves_sim_sk; [exact SIMSK|exact IH1|..]; eauto. i; des.
-    esplits; eauto.
-    - eapply link_list_cons; eauto.
-    - eapply link_list_cons; eauto.
-  Qed.
-
-  Corollary sim_load
-        sem_src
-        (LOADSRC: load p_src = Some sem_src)
-    :
-      exists sem_tgt, <<LOADTGT: load p_tgt = Some sem_tgt>>
-  .
-  Proof.
-    unfold load in *.
-    des_ifs_safe.
-    exploit sim_link_sk; eauto. i; des.
-    esplits; eauto. des_ifs.
-  Qed.
+(*   Variable pp: ProgPair.t. *)
+(*   Hypothesis SIMPROG: ProgPair.sim pp. *)
+(*   Let p_src := pp.(ProgPair.src). *)
+(*   Let p_tgt := pp.(ProgPair.tgt). *)
 
 
-End SIM.
+
+(*   Theorem sim_link_sk *)
+(*           sk_link_src *)
+(*           (LOADSRC: p_src.(link_sk) = Some sk_link_src) *)
+(*     : *)
+(*       exists ss_link sk_link_tgt, *)
+(*         <<LOADTGT: p_tgt.(link_sk) = Some sk_link_tgt>> *)
+(*         /\ <<LINKSS: pp.(ProgPair.ss_link) = Some ss_link>>  *)
+(*         /\ <<SIMSK: SimSymb.sim_sk ss_link sk_link_src sk_link_tgt>> *)
+(*   . *)
+(*   Proof. *)
+(*     u. subst_locals. *)
+(*     ginduction pp; ii; ss. *)
+(*     eapply link_list_cons_inv in LOADSRC. des. *)
+(*     inv SIMPROG. *)
+(*     exploit IHt; eauto. intro IH; des. *)
+(*     inv H1. *)
+(*     rename sk_link_src into sk_link_link_src. *)
+(*     rename restl into sk_link_src. *)
+(*     exploit SimSymb.sim_sk_weak_enables_link; eauto. *)
+(*     { eapply SimSymb.sim_sk_sim_sk_weak; eauto. } *)
+(*     { eapply SimSymb.sim_sk_sim_sk_weak; eauto. } *)
+(*     i; des. *)
+(*     exploit SimSymb.link_preserves_sim_sk; [exact SIMSK|exact IH1|..]; eauto. i; des. *)
+(*     esplits; eauto. *)
+(*     - eapply link_list_cons; eauto. *)
+(*     - eapply link_list_cons; eauto. *)
+(*   Qed. *)
+
+(*   Corollary sim_load *)
+(*         sem_src *)
+(*         (LOADSRC: load p_src = Some sem_src) *)
+(*     : *)
+(*       exists sem_tgt, <<LOADTGT: load p_tgt = Some sem_tgt>> *)
+(*   . *)
+(*   Proof. *)
+(*     unfold load in *. *)
+(*     des_ifs_safe. *)
+(*     exploit sim_link_sk; eauto. i; des. *)
+(*     esplits; eauto. des_ifs. *)
+(*   Qed. *)
+
+
+(* End SIM. *)
 
 
 
